fowl/Is/Injective.v
@@ -1,19 +1,135 @@
-(** * Injectivity *)
+(** * Injectivity and Cancellativity *)
 
 From DEZ Require Export
   Init.
 
-Class IsInjGen (A B C D : Type) (X : C -> D -> Prop) (Y : A -> B -> Prop)
-  (f : A -> C) (g : B -> D) : Prop :=
-  inj_gen (x : A) (y : B) (a : X (f x) (g y)) : Y x y.
-
 (** ** Injective Function *)
 
-Class IsInj2 (A B : Type) (X : B -> B -> Prop) (Y : A -> A -> Prop)
+Class IsInjFn (A B : Type) (X : A -> A -> Prop) (Y : B -> B -> Prop)
   (f : A -> B) : Prop :=
-  inj2 (x y : A) (a : X (f x) (f y)) : Y x y.
+  inj_fn (x y : A) (a : Y (f x) (f y)) : X x y.
 
-(** ** Injective Operation *)
+(** ** Cancellative Unary Operation *)
+(** ** Injective Unary Operation *)
 
 Class IsInj (A : Type) (X : A -> A -> Prop) (f : A -> A) : Prop :=
   inj (x y : A) (a : X (f x) (f y)) : X x y.
+
+Section Context.
+
+Context (A : Type) (X : A -> A -> Prop) (f : A -> A).
+
+(** Injectivity of a function implies its injectivity as a binary operation. *)
+
+#[export] Instance inj_fn_is_inj
+  `{!IsInjFn X X f} : IsInj X f.
+Proof. auto. Qed.
+
+(** Injectivity of a binary operation implies its injectivity as a function. *)
+
+#[local] Instance inj_is_inj_fn
+  `{!IsInj X f} : IsInjFn X X f.
+Proof. auto. Qed.
+
+End Context.
+
+(** ** Left Cancellative Form *)
+(** ** Left Injective Form *)
+
+Class IsCancelFormL (A B : Type) (X : A -> A -> Prop) (Y : B -> B -> Prop)
+  (s : A -> A -> B) : Prop :=
+  cancel_form_l (x y z : A) (a : Y (s x y) (s x z)) : X y z.
+
+(** ** Left Cancellative Form *)
+(** ** Left Injective Form *)
+
+Class IsCancelFormR (A B : Type) (X : A -> A -> Prop) (Y : B -> B -> Prop)
+  (s : A -> A -> B) : Prop :=
+  cancel_form_r (x y z : A) (a : Y (s x z) (s y z)) : X x y.
+
+(** ** Cancellative Form *)
+
+Class IsCancelForm (A B : Type) (X : A -> A -> Prop) (Y : B -> B -> Prop)
+  (s : A -> A -> B) : Prop := {
+  cancel_form_is_cancel_form_l :> IsCancelFormL X Y s;
+  cancel_form_is_cancel_form_r :> IsCancelFormR X Y s;
+}.
+
+(** ** Left Cancellative Binary Operation *)
+(** ** Left Injective Binary Operation *)
+
+(** This has the same shape as [Pos.add_reg_l]. *)
+
+Class IsCancelL (A : Type) (X : A -> A -> Prop) (k : A -> A -> A) : Prop :=
+  cancel_l (x y z : A) (a : X (k x y) (k x z)) : X y z.
+
+(** ** Right Cancellative Binary Operation *)
+(** ** Right Injective Binary Operation *)
+
+(** This has the same shape as [Pos.add_reg_r]. *)
+
+Class IsCancelR (A : Type) (X : A -> A -> Prop) (k : A -> A -> A) : Prop :=
+  cancel_r (x y z : A) (a : X (k x z) (k y z)) : X x y.
+
+(** ** Cancellative Binary Operation *)
+
+Class IsCancel (A : Type) (X : A -> A -> Prop) (k : A -> A -> A) : Prop := {
+  cancel_is_cancel_l :> IsCancelL X k;
+  cancel_is_cancel_r :> IsCancelR X k;
+}.
+
+Section Context.
+
+Context (A : Type) (X : A -> A -> Prop) (k : A -> A -> A).
+
+(** We cannot declare these definitions to be instances
+    until the end of this section if we want to avoid cycles. *)
+
+(** Left cancellative form implies left cancellative binary operation. *)
+
+Lemma cancel_form_l_is_cancel_l
+  `{!IsCancelFormL X X k} : IsCancelL X k.
+Proof. auto. Qed.
+
+(** Left cancellative binary operation implies left cancellative form. *)
+
+Lemma cancel_l_is_cancel_form_l
+  `{!IsCancelL X k} : IsCancelFormL X X k.
+Proof. auto. Qed.
+
+(** Right cancellative form implies right cancellative binary operation. *)
+
+Lemma cancel_form_r_is_cancel_r
+  `{!IsCancelFormR X X k} : IsCancelR X k.
+Proof. auto. Qed.
+
+(** Right cancellative binary operation implies right cancellative form. *)
+
+Lemma cancel_r_is_cancel_form_r
+  `{!IsCancelR X k} : IsCancelFormR X X k.
+Proof. auto. Qed.
+
+(** Cancellative form implies cancellative binary operation. *)
+
+#[export] Instance cancel_form_is_cancel
+  `{!IsCancelForm X X k} : IsCancel X k.
+Proof.
+  esplit; eauto
+  using cancel_form_l_is_cancel_l, cancel_form_r_is_cancel_r
+  with typeclass_instances. Qed.
+
+(** Cancellative binary operation implies cancellative form. *)
+
+#[local] Instance cancel_is_cancel_form
+  `{!IsCancel X k} : IsCancelForm X X k.
+Proof.
+  esplit; eauto
+  using cancel_l_is_cancel_form_l, cancel_r_is_cancel_form_r
+  with typeclass_instances. Qed.
+
+#[export] Existing Instance cancel_form_l_is_cancel_l.
+#[local] Existing Instance cancel_l_is_cancel_form_l.
+#[export] Existing Instance cancel_form_r_is_cancel_r.
+#[local] Existing Instance cancel_r_is_cancel_form_r.
+
+End Context.
