fowl/Is/Invertible.v
@@ -18,50 +18,50 @@ Class IsInvBinFnR (A B C : Type) (X : C -> C -> Prop)
 (** ** Left Invertible Form *)
 
 Class IsInvFormL (A B : Type) (X : B -> B -> Prop)
-  (x : B) (f : A -> A) (a : A -> A -> B) : Prop :=
-  inv_form_l (y : A) : X (a (f y) y) x.
+  (x : B) (f : A -> A) (s : A -> A -> B) : Prop :=
+  inv_form_l (y : A) : X (s (f y) y) x.
 
 (** ** Right Invertible Form *)
 
 Class IsInvFormR (A B : Type) (X : B -> B -> Prop)
-  (x : B) (f : A -> A) (a : A -> A -> B) : Prop :=
-  inv_form_r (y : A) : X (a y (f y)) x.
+  (x : B) (f : A -> A) (s : A -> A -> B) : Prop :=
+  inv_form_r (y : A) : X (s y (f y)) x.
 
 (** ** Invertible Form *)
 
 Class IsInvForm (A B : Type) (X : B -> B -> Prop)
-  (x : B) (f : A -> A) (a : A -> A -> B) : Prop := {
-  inv_form_is_inv_form_l :> IsInvFormL X x f a;
-  inv_form_is_inv_form_r :> IsInvFormR X x f a;
+  (x : B) (f : A -> A) (s : A -> A -> B) : Prop := {
+  inv_form_is_inv_form_l :> IsInvFormL X x f s;
+  inv_form_is_inv_form_r :> IsInvFormR X x f s;
 }.
 
 Section Context.
 
 Context (A : Type) (X : A -> A -> Prop)
-  (x : A) (f : A -> A) (a : A -> A -> A).
+  (x : A) (f : A -> A) (s : A -> A -> A).
 
 (** Left invertible binary function implies left invertible form. *)
 
 #[export] Instance inv_bin_fn_l_is_inv_form_l
-  `{!IsInvBinFnL X x f a} : IsInvFormL X x f a.
+  `{!IsInvBinFnL X x f s} : IsInvFormL X x f s.
 Proof. auto. Qed.
 
 (** Left invertible form implies left invertible binary function. *)
 
 #[local] Instance inv_form_l_is_inv_bin_fn_l
-  `{!IsInvFormL X x f a} : IsInvBinFnL X x f a.
+  `{!IsInvFormL X x f s} : IsInvBinFnL X x f s.
 Proof. auto. Qed.
 
 (** Right invertible binary function implies right invertible form. *)
 
 #[export] Instance inv_bin_fn_r_is_inv_form_r
-  `{!IsInvBinFnR X x f a} : IsInvFormR X x f a.
+  `{!IsInvBinFnR X x f s} : IsInvFormR X x f s.
 Proof. auto. Qed.
 
 (** Right invertible form implies right invertible binary function. *)
 
 #[local] Instance inv_form_r_is_inv_bin_fn_r
-  `{!IsInvFormR X x f a} : IsInvBinFnR X x f a.
+  `{!IsInvFormR X x f s} : IsInvBinFnR X x f s.
 Proof. auto. Qed.
 
 End Context.
@@ -95,10 +95,10 @@ Section Context.
 Context (A : Type) (X : A -> A -> Prop)
   (x : A) (f : A -> A) (k : A -> A -> A).
 
-(** Left invertible form implies left invertible binary operation. *)
-
 (** We cannot declare these definitions to be instances
     until the end of this section if we want to avoid cycles. *)
+
+(** Left invertible form implies left invertible binary operation. *)
 
 Lemma inv_form_l_is_inv_l
   `{!IsInvFormL X x f k} : IsInvL X x f k.
@@ -122,7 +122,7 @@ Lemma inv_r_is_inv_form_r
   `{!IsInvR X x f k} : IsInvFormR X x f k.
 Proof. auto. Qed.
 
-(** Invertible binary function implies invertible form. *)
+(** Invertible form implies invertible binary operation. *)
 
 #[export] Instance inv_form_is_inv
   `{!IsInvForm X x f k} : IsInv X x f k.
@@ -131,7 +131,7 @@ Proof.
   using inv_form_l_is_inv_l, inv_form_r_is_inv_r
   with typeclass_instances. Qed.
 
-(** Invertible form implies invertible binary function. *)
+(** Invertible binary operation implies invertible form. *)
 
 #[local] Instance inv_is_inv_form
   `{!IsInv X x f k} : IsInvForm X x f k.
