fowl/Has/CategoricalOperations.v
@@ -10,6 +10,8 @@ From DEZ.Supports Require Import
 Class HasIdHom (A : Type) {X : HasHom A} : Type :=
   id_hom (x : A) : x --> x.
 
+Arguments HasIdHom _ {_}.
+
 #[export] Typeclasses Transparent HasIdHom.
 
 (** ** Inverse Morphism *)
@@ -17,11 +19,15 @@ Class HasIdHom (A : Type) {X : HasHom A} : Type :=
 Class HasInvHom (A : Type) {X : HasHom A} : Type :=
   inv_hom (x y : A) (a : x --> y) : y --> x.
 
+Arguments HasInvHom _ {_}.
+
 #[export] Typeclasses Transparent HasInvHom.
 
 (** ** Composed Morphism *)
 
 Class HasCompHom (A : Type) {X : HasHom A} : Type :=
   comp_hom (x y z : A) (a : y --> z) (b : x --> y) : x --> z.
+
+Arguments HasCompHom _ {_}.
 
 #[export] Typeclasses Transparent HasCompHom.
