fowl/Is/Monoid.v
@@ -1,7 +1,7 @@
 (** * Monoidal Structure *)
 
 From DEZ.Is Require Export
-  Semigroup Unital.
+  Semigroup Unital Associative.
 
 (** ** Monoid *)
 
@@ -10,13 +10,3 @@ Class IsMon (A : Type) (X : A -> A -> Prop)
   mon_is_semigrp :> IsSemigrp X k;
   mon_is_unl :> IsUnl X x k;
 }.
-
-Section Context.
-
-Context (A : Type) (X : A -> A -> Prop)
-  (x : A) (k : A -> A -> A) `{!IsMon X x k}.
-
-#[local] Instance mon_is_assoc : IsAssoc X k.
-Proof. typeclasses eauto. Qed.
-
-End Context.
