fowl/Is/Semiring.v
@@ -1,11 +1,7 @@
 (** * Semiring Structure *)
 
-From DEZ.Has Require Export
-  EquivalenceRelation Zero Addition One Multiplication.
 From DEZ.Is Require Export
-  Monoid Commutative Distributive Absorbing Truncated.
-From DEZ.Supports Require Import
-  EquivalenceNotations ArithmeticNotations.
+  Monoid Commutative Distributive Absorbing.
 
 (** ** Semiring *)
 
@@ -17,50 +13,3 @@ Class IsSemiring (A : Type) (X : A -> A -> Prop)
   semiring_is_distr :> IsDistr X m k;
   semiring_is_absorb_elem :> IsAbsorbElem X x m;
 }.
-
-Section Context.
-
-Context (A : Type) (X : A -> A -> Prop)
-  (x : A) (k : A -> A -> A) (y : A) (m : A -> A -> A) `{!IsSemiring X x k y m}.
-
-#[local] Instance has_equiv_rel : HasEquivRel A := X.
-#[local] Instance has_zero : HasZero A := x.
-#[local] Instance has_add : HasAdd A := k.
-#[local] Instance has_one : HasOne A := y.
-#[local] Instance has_mul : HasMul A := m.
-
-Ltac note := progress (
-  try change X with equiv_rel in *;
-  try change x with zero in *;
-  try change k with add in *;
-  try change y with one in *;
-  try change m with mul in *).
-
-(** TODO Does this make sense anymore? *)
-
-Import Zero.Subclass Negation.Subclass Addition.Subclass
-  One.Subclass Multiplication.Subclass.
-
-Ltac subclass := progress (
-  try change bin_rel with equiv_rel in *;
-  try change null_op with zero in *;
-  try change bin_op with add in *;
-  try change null_op with one in *;
-  try change bin_op with mul in *).
-
-#[local] Instance is_contr (a : X 0 1) : IsContr X.
-Proof.
-  hnf.
-  note.
-  exists 0.
-  intros z.
-  assert (b : z * 0 == z * 1).
-  { apply (proper : IsProper (_==_ ==> _==_ ==> _==_) _*_); easy. }
-  setoid_rewrite (unl_r z) in b.
-  setoid_rewrite (absorb_elem_r z) in b.
-  setoid_rewrite b.
-  reflexivity. Qed.
-
-End Context.
-
-#[export] Hint Resolve is_contr : typeclass_instances.
